to_simple_ruleset

SemanticsTernary/pfprefix_PF_To_Iptables.thy
@@ -373,14 +373,53 @@ definition pfcp_to_iptcp_rs :: "pfprefix_Primitives.common_primitive ruleset \<R
 "pfcp_to_iptcp_rs = map (\<lambda>l. (case l of (PfRule r) \<Rightarrow> (Rule (pfm_to_iptm (pf_rule.get_match r)) (pfa_to_ipta (pf_rule.get_action r)))))"
 
 fun pf_to_ipt :: "pfcontext \<Rightarrow> pfprefix_Primitives.common_primitive ruleset \<Rightarrow> 32 common_primitive rule list" where
-"pf_to_ipt ctx rs = pfcp_to_iptcp_rs (rev (normalize_ports_rs (remove_tables_rs ctx (remove_quick' (remove_matches (remove_anchors' rs))))))"
+"pf_to_ipt ctx rs = pfcp_to_iptcp_rs (rev (normalize_ports_rs (remove_tables_rs ctx (remove_quick_approx (remove_matches (remove_anchors' rs))))))"
 
 
 fun pf_decision_to_ipt_decision :: "decision \<Rightarrow> state" where
 "pf_decision_to_ipt_decision decision.Accept = Decision FinalAllow" |
 "pf_decision_to_ipt_decision decision.Reject = Decision FinalDeny"
 
-theorem "pf_decision_to_ipt_decision
+definition to_simple_ruleset :: "'a line list \<Rightarrow> 'a line list" where
+"to_simple_ruleset rs = remove_quick_approx (remove_matches (remove_anchors' rs))"
+
+lemma
+  assumes "no_match_quick rs"
+      and "no_unknown_anchors (pfprefix_PrimitiveMatchers.common_matcher ctx, pfprefix_Unknown_Match_Tacs.in_doubt_allow) rs"
+  shows
+ "pf_approx rs (pfprefix_PrimitiveMatchers.common_matcher ctx, pfprefix_Unknown_Match_Tacs.in_doubt_allow) p =
+  pf_approx (to_simple_ruleset rs) (pfprefix_PrimitiveMatchers.common_matcher ctx, pfprefix_Unknown_Match_Tacs.in_doubt_allow) p"
+  and "simple_ruleset (to_simple_ruleset rs)"
+proof(-)
+  have *: "(pf_approx rs (pfprefix_PrimitiveMatchers.common_matcher ctx, pfprefix_Unknown_Match_Tacs.in_doubt_allow) p) =
+        (pf_approx (remove_anchors' rs) (pfprefix_PrimitiveMatchers.common_matcher ctx, pfprefix_Unknown_Match_Tacs.in_doubt_allow) p)"
+    (is "?original = pf_approx (?anchors_removed) ?m ?p")
+    using assms by (simp add:remove_anchors'_preserves_semantics)
+  have na:"no_anchors ?anchors_removed" by (simp add:remove_anchors'_ok)
+  have nmq:"no_match_quick ?anchors_removed" using assms remove_anchors'_preserves_no_match_quick by blast
+  have *: "?original = pf_approx (remove_matches ?anchors_removed) ?m ?p"
+(is "?original = pf_approx (?matches_removed) ?m ?p")
+    using * na nmq assms by(auto simp add:remove_matches_preserves_semantics)
+  have nm:"no_match ?matches_removed" using na nmq remove_matches_ok by blast
+  have na:"no_anchors ?matches_removed" using na using remove_matches_preserves_no_anchors by blast
+  have gm:"good_matcher ?m" by (simp add:in_doubt_allow_good_matcher)
+  have *: "?original = pf_approx (remove_quick_approx ?matches_removed) ?m ?p"
+    (is "?original = pf_approx (?quick_removed) ?m ?p")
+    using * na nm gm assms by(simp add:remove_quick_approx_preserves_semantics)
+  then show "pf_approx rs (pfprefix_PrimitiveMatchers.common_matcher ctx, pfprefix_Unknown_Match_Tacs.in_doubt_allow) p =
+  pf_approx (to_simple_ruleset rs) (pfprefix_PrimitiveMatchers.common_matcher ctx, pfprefix_Unknown_Match_Tacs.in_doubt_allow) p" 
+    unfolding to_simple_ruleset_def by simp
+  have nq:"no_quick ?quick_removed" using na remove_quick_approx_ok by blast
+  have nm:"no_match ?quick_removed" using na nm remove_quick_approx_preserves_no_match by blast
+  have na:"no_anchors ?quick_removed" using na remove_quick_approx_preserves_no_anchors by blast
+  from nq nm na show "simple_ruleset (to_simple_ruleset rs)" unfolding to_simple_ruleset_def by (simp add:simple_ruleset_def)
+qed
+
+theorem
+  assumes "no_match_quick rs"
+      and "no_unknown_anchors (pfprefix_PrimitiveMatchers.common_matcher ctx, pfprefix_Unknown_Match_Tacs.in_doubt_allow) rs"
+  shows
+ "pf_decision_to_ipt_decision
  (pf_approx rs (pfprefix_PrimitiveMatchers.common_matcher ctx, pfprefix_Unknown_Match_Tacs.in_doubt_allow) (tagged_packet_untag p)) =
 approximating_bigstep_fun (common_matcher,in_doubt_allow) p (pf_to_ipt ctx rs) Undecided"
   sorry
